minor: progress

CoqOfRust/plonky3/blake3-air/link/air.v
@@ -4,8 +4,31 @@ Require Import plonky3.blake3-airsrc.air.
 
 (* pub struct Blake3Air {} *)
 
+(* TODO: refer to `opcode` in revm *)
 (* TODO: check if the name of the module fits in the style with other translated links *)
 Module Impl_Blake3Air.
+  Inductive t : Set := .
+
+(* 
+  Global Instance IsLink : Link t := {
+    Φ := Ty.path "revm_context_interface::cfg::CreateScheme";
+    φ x :=
+      match x with
+      | Create => Value.StructTuple "revm_context_interface::cfg::CreateScheme::Create" []
+      | Create2 x =>
+        Value.StructRecord "revm_context_interface::cfg::CreateScheme::Create2" [
+          ("salt", φ x)
+        ]
+      end;
+  }.
+
+  Definition of_ty : OfTy.t (Ty.path "revm_context_interface::cfg::CreateScheme").
+  Proof. eapply OfTy.Make with (A := t); reflexivity. Defined.
+  Smpl Add apply of_ty : of_ty.
+
+*)
+
+
 End Impl_Blake3Air.
 (* 
 impl Blake3Air {
@@ -14,4 +37,16 @@ impl Blake3Air {
         num_hashes: usize,
         extra_capacity_bits: usize,
     ) -> RowMajorMatrix<F> {
+*)
+
+(* 
+Module Impl_Transaction_for_Ref_Transaction.
+  Instance run
+    (Self : Set) `{Link Self}
+    (types : Transaction.Types.t) `{Transaction.Types.AreLinks types}
+    (run_Transaction_for_Self : Transaction.Run Self types) :
+    Transaction.Run (Ref.t Pointer.Kind.Ref Self) types.
+  Admitted.
+End Impl_Transaction_for_Ref_Transaction.
+
 *)
